Tracking access to left symbols in blame
A possible reason for the failure of attempts to modify the memory
associated to a block on the left side of an injection is that these
blocks necessarily are "placeholders" to function definitions, and
their permissions prevent the hypothesized success of various memory
operations, thus creating a contradiction.

security/Blame.v
@@ -250,11 +250,135 @@ Section Equivalence.
       eapply same_blocks_store; eauto.
   Qed.
 
-  Definition symbols_inject_left f ge1 ge2 (cp: compartment) :=
+  Definition symbols_inject_left f (ge1 ge2: genv) m cp :=
     forall id b1 b2 delta,
       f b1 = Some (b2, delta) ->
-      Senv.find_symbol ge1 id = Some b1 ->
-      delta = 0 /\ Senv.find_symbol ge2 id = Some b2.
+      Genv.find_symbol ge1 id = Some b1 ->
+      Genv.find_comp_of_block ge1 b1 = Some cp ->
+      delta = 0 /\ Senv.find_symbol ge2 id = Some b2 /\
+      (Mem.mem_access m) !! b1 delta Cur = Some Nonempty.
+
+  (* TODO It would be nice to avoid these low-level helpers *)
+  Lemma mem_access_free_1:
+    forall m1 bf lo hi cp m2,
+    Mem.free m1 bf lo hi cp = Some m2 ->
+    forall b ofs k,
+    b <> bf \/ ofs < lo \/ hi <= ofs ->
+    (Mem.mem_access m1) !! b ofs k = (Mem.mem_access m2) !! b ofs k.
+  Proof.
+    clear.
+    intros.
+Local Transparent Mem.free. unfold Mem.free in H. Local Opaque Mem.free.
+    destruct Mem.range_perm_dec; [| discriminate].
+    destruct Mem.can_access_block_dec; [| discriminate].
+    injection H as <-.
+    unfold Mem.unchecked_free.
+    destruct zle; [reflexivity |].
+    simpl. rewrite PMap.gsspec.
+    destruct peq; [subst b | reflexivity].
+    destruct H0 as [| H0]; [contradiction |].
+    destruct H0 as [H0 | H0].
+    - destruct (zle lo ofs); [lia |]. reflexivity.
+    - destruct (zlt ofs hi); [lia |]. rewrite andb_false_r. reflexivity.
+  Qed.
+
+  (* TODO It would be nice to avoid these low-level helpers *)
+  Lemma mem_access_free_inv:
+    forall m1 bf lo hi cp m2,
+    Mem.free m1 bf lo hi cp = Some m2 ->
+    forall b ofs k p,
+    (Mem.mem_access m1) !! b ofs k = Some p ->
+    b = bf /\ lo <= ofs < hi \/ (Mem.mem_access m2) !! b ofs k = Some p.
+  Proof.
+    clear.
+    intros. exploit Mem.free_result; eauto. intros. subst m2.
+    unfold Mem.unchecked_free; destruct (zle hi lo); auto; simpl.
+    rewrite PMap.gsspec. destruct (peq b bf); auto. subst b.
+    destruct (zle lo ofs); simpl; auto.
+    destruct (zlt ofs hi); simpl; auto.
+  Qed.
+
+  (* TODO It would be nice to avoid these low-level helpers *)
+  Lemma mem_access_alloc_1:
+    forall m1 c lo hi m2 b,
+    Mem.alloc m1 c lo hi = (m2, b) ->
+    forall b' ofs k,
+    b' <> b ->
+    (Mem.mem_access m1) !! b' ofs k = (Mem.mem_access m2) !! b' ofs k.
+  Proof.
+    clear.
+    intros.
+Local Transparent Mem.alloc. unfold Mem.alloc in H. Local Opaque Mem.alloc.
+    injection H as <- <-.
+    simpl. rewrite PMap.gso; auto.
+  Qed.
+
+  Lemma symbols_inject_left_free m b lo hi cp m' ge1 ge2 cp'
+    (FREE : Mem.free m b lo hi cp = Some m')
+    (SYMB : symbols_inject_left j ge1 ge2 m cp') :
+    symbols_inject_left j ge1 ge2 m' cp'.
+  Proof.
+    (* destruct SYMB as [FIND ACC]. split; [exact FIND |]. *)
+    intros id b1 b2 ofs b1_b2 FIND1 COMP1.
+    specialize (SYMB _ _ _ _ b1_b2 FIND1 COMP1) as (-> & FIND2 & ACC).
+    split; [reflexivity |]. split; [exact FIND2 |].
+    destruct (peq b1 b) as [-> | NEQ].
+    - destruct (mem_access_free_inv _ _ _ _ _ _ FREE _ _ _ _ ACC)
+        as [[_ RANGE] | PERM]; [| exact PERM].
+Local Transparent Mem.free. unfold Mem.free in FREE. Local Opaque Mem.free.
+      destruct Mem.range_perm_dec; [| discriminate].
+      assert (PERM := r). specialize (PERM _ RANGE).
+      unfold Mem.perm, Mem.perm_order' in PERM. rewrite ACC in PERM.
+      inv PERM.
+    - erewrite <- mem_access_free_1; eauto.
+  Qed.
+
+  Lemma symbols_inject_left_free_list m bs cp m' ge1 ge2 cp'
+    (FREE : Mem.free_list m bs cp = Some m')
+    (SYMB : symbols_inject_left j ge1 ge2 m cp') :
+    symbols_inject_left j ge1 ge2 m' cp'.
+  Proof.
+    revert m cp m' ge1 ge2 cp' FREE SYMB.
+    induction bs as [| [[b lo] hi] ? IH]; intros.
+    - now inv FREE.
+    - simpl in FREE.
+      destruct (Mem.free m b lo hi cp) as [m1 |] eqn:FREE1; [| discriminate].
+      eapply symbols_inject_left_free in FREE1; eauto.
+  Qed.
+
+  Lemma symbols_inject_left_store chunk m b ofs sz cp m' ge1 ge2 cp'
+    (STORE : Mem.store chunk m b ofs sz cp = Some m')
+    (SYMB : symbols_inject_left j ge1 ge2 m cp') :
+    symbols_inject_left j ge1 ge2 m' cp'.
+  Proof.
+    intros id b1 b2 ofs' b1_b2 id_b1 b1_cp'.
+    specialize (SYMB _ _ _ _ b1_b2 id_b1 b1_cp') as (-> & id_b2 & m'_b1).
+    split; [| split]; auto.
+    erewrite Mem.store_access; eauto.
+  Qed.
+
+  Lemma symbols_inject_left_storebytes m b ofs sz ocp m' ge1 ge2 cp
+    (STORE : Mem.storebytes m b ofs sz ocp = Some m')
+    (SYMB : symbols_inject_left j ge1 ge2 m cp) :
+    symbols_inject_left j ge1 ge2 m' cp.
+  Proof.
+    intros id b1 b2 ofs' b1_b2 id_b1 b1_cp.
+    specialize (SYMB _ _ _ _ b1_b2 id_b1 b1_cp) as (-> & id_b2 & m'_b1).
+    split; [| split]; auto.
+    erewrite Mem.storebytes_access; eauto.
+  Qed.
+
+  Lemma symbols_inject_left_assign_loc {ce cp ty m b ofs bf v m' ge1 ge2 cp'}
+    (ASSIGN : assign_loc ce cp ty m b ofs bf v m')
+    (SYMB : symbols_inject_left j ge1 ge2 m cp') :
+    symbols_inject_left j ge1 ge2 m' cp'.
+  Proof.
+    inv ASSIGN.
+    - eapply symbols_inject_left_store; eauto.
+    - eapply symbols_inject_left_storebytes; eauto.
+    - inv H.
+      eapply symbols_inject_left_store; eauto.
+  Qed.
 
   Record right_mem_injection (ge1 ge2: genv) (m1 m2: mem) : Prop :=
     { same_dom: same_domain_right ge1 m1;
@@ -265,7 +389,7 @@ Section Equivalence.
          public symbol must be covered by the memory injection. *)
       (* TODO replace symbols_inject with meminj_preserves_globals *)
       same_symb: forall cp, s cp = Right -> symbols_inject j ge1 ge2 (Genv.find_comp_of_ident ge1) cp;
-      same_symb_left: forall cp, s cp = Left -> symbols_inject_left j ge1 ge2 cp;
+      same_symb_left: forall cp, s cp = Left -> symbols_inject_left j ge1 ge2 m1 cp;
       same_blks1: same_blocks ge1 m1;
       same_blks2: same_blocks ge2 m2;
     }.
@@ -1179,7 +1303,7 @@ Lemma right_mem_injection_free: forall {j ge1 ge2 m1 m2 b1 b2 lo hi cp m1'},
     right_mem_injection s j ge1 ge2 m1' m2'.
 Proof.
   intros j ge1 ge2 m1 m2 b1 b2 lo hi cp m1' MEMINJ FREE1 j_b1.
-  destruct MEMINJ as [DOM MI D0 SYMB BLKS1 BLKS2].
+  destruct MEMINJ as [DOM MI D0 SYMB SYMBL BLKS1 BLKS2].
   pose proof (Mem.free_range_perm _ _ _ _ _ _ FREE1) as RANGE1.
   pose proof (Mem.free_can_access_block_1 _ _ _ _ _ _ FREE1) as ACCESS1.
   assert (Mem.range_perm m2 b2 lo hi Cur Freeable) as RANGE2.
@@ -1197,6 +1321,17 @@ Proof.
   - eauto using same_domain_right_free.
   - exploit Mem.free_parallel_inject; eauto.
     rewrite !Z.add_0_r. intros (? & ? & ?). congruence.
+  - intros cp' LEFT id b1' b2' ofs b1'_b2' id_b1' b1'_cp'.
+    specialize (SYMBL _ LEFT _ _ _ _ b1'_b2' id_b1' b1'_cp') as (-> & FINDL & PERML).
+    split; [reflexivity |]. split; [eassumption |].
+    destruct (peq b1' b1) as [-> | NEQ].
+    + rewrite j_b1 in b1'_b2'. injection b1'_b2' as <-.
+      destruct (mem_access_free_inv _ _ _ _ _ _ FREE1 _ _ _ _ PERML)
+        as [[_ RANGE] | PERM]; [| exact PERM].
+      specialize (RANGE1 _ RANGE).
+      unfold Mem.perm, Mem.perm_order' in RANGE1. rewrite PERML in RANGE1.
+      inv RANGE1.
+    + erewrite <- mem_access_free_1; eauto.
   - eapply same_blocks_free; eauto.
   - eapply same_blocks_free; eauto.
 Qed.
@@ -1246,10 +1381,11 @@ Lemma right_mem_injection_free_list_left:
     right_mem_injection s j ge1 ge2 m1' m2.
 Proof.
   intros.
-  destruct RMEMINJ as [DOM MI D0 SYMB BLKS1 BLKS2].
+  destruct RMEMINJ as [DOM MI D0 SYMB SYMBL BLKS1 BLKS2].
   split; trivial.
   - eauto using same_domain_right_free_list.
   - eauto using Mem.free_list_left_inject.
+  - eauto using symbols_inject_left_free_list.
   - eauto using same_blocks_free_list.
 Qed.
 
@@ -1610,7 +1746,8 @@ Admitted.
             destruct (Mem.block_compartment m1 b1) as [cp' |] eqn:COMP ; [| contradiction].
             erewrite same_blks1 in COMP; eauto. congruence.
           + exploit right_mem_injection_right; eauto. intros (cp' & COMP & _).
-            exploit same_symb_left; eauto. easy.
+            exploit same_symb_left; eauto. intros (-> & SYMBL & ACCL).
+            easy.
         - destruct (Mem.block_compartment m1 b1) as [cp' |] eqn:COMP.
           + exploit same_symb; eauto.
             intros (H1 & H2 & H3 & H4).
@@ -1631,8 +1768,8 @@ Admitted.
         * rewrite Genv.globalenv_policy in imp, exp. rewrite Genv.globalenv_policy.
           simpl. rewrite (match_prog_pol _ _ _ match_W1_W2).
           apply Genv.invert_find_symbol in ge1_b1.
-          destruct (same_symb_left _ _ _ _ _ _ inj _ SIDE _ _ _ _ j_b1 ge1_b1)
-            as (-> & ge2_b2).
+          destruct (same_symb_left _ _ _ _ _ _ inj _ SIDE _ _ _ _ j_b1 ge1_b1 ge1_b1')
+            as (-> & ge2_b2 & m1_b1).
           split; [| split].
           -- apply Genv.find_invert_symbol in ge2_b2. assumption.
           -- exploit find_comp_of_block_preserved; eauto.
@@ -1682,7 +1819,9 @@ Admitted.
         unfold Genv.find_comp_of_ident in id_cp. setoid_rewrite FIND1 in id_cp.
         erewrite same_blks1 in COMP; eauto. injection COMP as <-. congruence.
       + exploit right_mem_injection_right; eauto. intros (cp' & COMP & _).
-        exploit same_symb_left; eauto. easy.
+        unfold Genv.find_comp_of_ident in id_cp. setoid_rewrite FIND1 in id_cp.
+        exploit same_symb_left; eauto. intros (-> & SYMBL & ACCL).
+        easy.
     - exploit same_symb; eauto.
       intros (_ & H & ?).
       now destruct (H id b1 b2 delta j_b1 FIND1) as [??].
@@ -1858,13 +1997,16 @@ Admitted.
              reflexivity.
           -- rewrite (EXT _ NEQ) in b1'_b2'.
              exact (VOL _ _ _ b1'_b2').
-      + intros cp' LEFT id' b1' b2' delta b1'_b2' ge1_b1'.
+      + intros cp' LEFT id' b1' b2' delta b1'_b2' id'_b1' b1'_cp'.
         assert (NEQ: b1' <> b1).
         { eapply Mem.valid_block_alloc_inv'; eauto.
-          clear -ge1_b1' BLKS1. simpl in *.
+          clear -id'_b1' BLKS1. simpl in *.
           exploit find_symbol_valid_block; eauto. }
-        rewrite (EXT _ NEQ) in b1'_b2'.
-        eapply SYMBL; eauto.
+        specialize (EXT _ NEQ). rewrite EXT in b1'_b2'.
+        specialize (SYMBL _ LEFT _ _ _ _ b1'_b2' id'_b1' b1'_cp')
+          as (-> & id'_b2' & m1_b1').
+        split; [reflexivity |]. split; [assumption |].
+        erewrite <- mem_access_alloc_1; eauto.
       + intros b cp' FIND. specialize (BLKS1 b cp' FIND).
         change (Mem.block_compartment _ _ = _)
           with (Mem.can_access_block m1' b (Some cp')).
@@ -1917,16 +2059,34 @@ Admitted.
       + intros [| [fd DEF]]; [discriminate |]. eauto.
   Qed.
 
+  Lemma symbols_inject_left_alloc_left :
+    forall j ge1 ge2 m cp lo hi cp' m' b,
+      symbols_inject_left j ge1 ge2 m cp ->
+      Mem.alloc m cp' lo hi = (m', b) ->
+      s cp = Left ->
+      symbols_inject_left j ge1 ge2 m' cp.
+  Proof.
+    intros j ge1 ge2 m cp lo hi cp' m' b j_m m_m' s_cp
+           id b1 b2 ofs b1_b2 id_b1 b1_cp.
+    specialize (j_m _ _ _ _ b1_b2 id_b1 b1_cp) as (-> & id_b2 & m_b1).
+    split; [| split]; auto.
+    assert (NEQ: b1 <> b).
+    { eapply Mem.valid_block_alloc_inv'; eauto.
+      eapply Genv.mem_access_valid_block; eauto. }
+    erewrite <- mem_access_alloc_1; eauto.
+  Qed.
+
   Lemma right_mem_injection_alloc_left {j cp m1 m2 m1' b1 lo hi}
     (RMEMINJ: right_mem_injection s j ge1 ge2 m1 m2)
     (LEFT: s cp = Left)
     (ALLOC: Mem.alloc m1 cp lo hi = (m1', b1)):
     right_mem_injection s j ge1 ge2 m1' m2.
   Proof.
-    destruct RMEMINJ as [DOM MI D0 SYMB BLKS1 BLKS2].
+    destruct RMEMINJ as [DOM MI D0 SYMB SYMBL BLKS1 BLKS2].
     split; trivial.
     - eauto using same_domain_right_alloc_left.
     - eauto using Mem.alloc_left_unmapped_inject_strong.
+    - eauto using symbols_inject_left_alloc_left.
     - eauto using same_blocks_alloc.
   Qed.
 
@@ -2012,7 +2172,7 @@ Admitted.
     exploit Mem.store_mapped_inject; eauto.
     rewrite Z.add_0_r. intros (m2' & STORE2 & INJ').
     exists m2'; split; trivial. constructor; trivial;
-    eauto using same_domain_right_store, same_blocks_store.
+    eauto using same_domain_right_store, same_blocks_store, symbols_inject_left_store.
   Qed.
 
   Lemma right_mem_injection_store_unmapped :
@@ -2027,7 +2187,7 @@ Admitted.
     exploit Mem.store_unmapped_inject; eauto.
     intros MI'.
     constructor; trivial;
-    eauto using same_domain_right_store, same_blocks_store.
+    eauto using same_domain_right_store, same_blocks_store, symbols_inject_left_store.
   Qed.
 
   Lemma right_mem_injection_store_outside :
@@ -2060,7 +2220,7 @@ Admitted.
     rewrite Z.add_0_r. intros (m2' & STORE2 & MI').
     exists m2'. split; trivial.
     constructor;
-    eauto using same_domain_right_storebytes, same_blocks_storebytes.
+    eauto using same_domain_right_storebytes, same_blocks_storebytes, symbols_inject_left_storebytes.
   Qed.
 
   Lemma right_mem_injection_storebytes_unmapped
@@ -2073,7 +2233,7 @@ Admitted.
     intros [DOM MI D0 SYMB BLKS1 BLKS2] LOCINJ STORE1.
     exploit Mem.storebytes_unmapped_inject; eauto. intros MI'.
     constructor;
-    eauto using same_domain_right_storebytes, same_blocks_storebytes.
+    eauto using same_domain_right_storebytes, same_blocks_storebytes, symbols_inject_left_storebytes.
   Qed.
 
   Lemma right_mem_injection_storebytes_outside
@@ -2127,7 +2287,7 @@ Qed.
     intros (m2' & ASSIGN2 & MEMINJ & LOAD).
     rewrite genv_cenv_preserved. exists m2'; split; trivial.
     destruct RMEMINJ as [DOM MI D0 SYMB BLKS1 BLKS2].
-    constructor; eauto using same_domain_right_assign_loc, same_blocks_assign_loc.
+    constructor; eauto using same_domain_right_assign_loc, same_blocks_assign_loc, symbols_inject_left_assign_loc.
   Qed.
 
   Lemma right_mem_injection_assign_loc_unmapped
@@ -2486,6 +2646,10 @@ Qed.
       apply DOM in j_b_undef. simpl in j_b_undef.
       rewrite m1_b in j_b_undef.
       destruct j_b_undef as [| [fd DEF]]; [congruence |].
+      admit.
+    - intros cp' LEFT' id b1 b2 ofs b1_b2 id_b1 b1_cp'.
+      specialize (SYMBL _ LEFT' _ _ _ _ b1_b2 id_b1 b1_cp') as (-> & id_b2 & m1_b1).
+      split; [| split]; auto.
       admit.
     - intros b cp ge_b. specialize (BLKS1 _ _ ge_b).
       enough (Mem.can_access_block m1' b (Some cp)) by easy.
@@ -4630,11 +4794,12 @@ Proof.
       setoid_rewrite DEF1. setoid_rewrite DEF2. reflexivity.
 Qed.
 
-Lemma symbols_inject_left_init_meminj cp'
+Lemma symbols_inject_left_init_meminj m1 cp'
+  (MEM1: Genv.init_mem W1 = Some m1)
   (LEFT': s cp' = Left):
-  symbols_inject_left init_meminj ge1 ge2 cp'.
+  symbols_inject_left init_meminj ge1 ge2 m1 cp'.
 Proof.
-  intros id b1 b2 ofs b1_b2 SYM1.
+  intros id b1 b2 ofs b1_b2 SYM1 COMP1.
   unfold init_meminj, init_meminj_block in b1_b2.
   (* Slightly modified standard processing *)
   apply Genv.find_invert_symbol in SYM1. rewrite SYM1 in b1_b2.
@@ -4650,11 +4815,16 @@ Proof.
     destruct (Genv.find_symbol ge2 id) as [b'' |] eqn:SYM2; [| discriminate].
     injection b1_b2 as -> <-.
     (* Done *)
-    auto.
+    split; [| split]; auto.
+    apply Genv.find_funct_ptr_iff in DEF1.
+    exploit Genv.init_mem_characterization_2'; eauto. intros (ACC1 & _).
+    rewrite ACC1, zeq_true. reflexivity.
   - destruct (Genv.find_symbol ge2 id) as [b' |] eqn:SYM2; [| discriminate].
     injection b1_b2 as -> <-.
     (* Done *)
-    auto.
+    apply Genv.invert_find_symbol in SYM1.
+    unfold Genv.find_comp_of_ident in COMP. setoid_rewrite SYM1 in COMP.
+    setoid_rewrite COMP1 in COMP. injection COMP as ->. congruence.
 Qed.
 
 Lemma initial_mem_injection m1 m2
@@ -4668,7 +4838,7 @@ Proof.
   - apply inject_init_meminj; assumption.
   - apply delta_zero_init_meminj.
   - apply symbols_inject_init_meminj.
-  - apply symbols_inject_left_init_meminj.
+  - intros. apply symbols_inject_left_init_meminj; assumption.
   - apply init_mem_same_blocks; assumption.
   - apply init_mem_same_blocks; assumption.
 Qed.
